\documentclass[a4paper]{article}

\usepackage{listings}
\usepackage{amsthm}
\usepackage{mathtools}

\DeclarePairedDelimiter\abs{\lvert}{\rvert}

\theoremstyle{plain}
\newtheorem{theorem}{Theorem}
\newtheorem{lemma}[theorem]{Lemma}

\theoremstyle{definition}
\newtheorem{definition}[theorem]{Definition}
\newtheorem{example}[theorem]{Example}
\newtheorem{remark}[theorem]{Remark}


\title{Fraction to float conversions}
\author{Mark Dickinson}

\begin{document}

\maketitle

\begin{theorem}
    Suppose that $a/b$ and $c/d$ are rational numbers, written in lowest terms
    (with $b$ and $d$ positive), that $\max(a, b, c, d) \le 67114657$, and that
    $a/b$ and $c/d$ become equal when rounded to the nearest finite IEEE
    binary64 floating-point number. Then $a/b = c/d$.
\end{theorem}

\begin{proof}
    It's straightforward to check that when we round a fraction with numerator
    and denominator bounded by~$67114657$ to a float, no underflow or overflow
    occurs, and that under the same bounds positive fractions round to positive
    floats and negative fractions to negative floats. So if $a/b$ and $c/d$
    round to the same float then both are positive, both are negative, or both
    are zero, and in the last case we're done. Negating both fractions if
    necessary, without loss of generality we can assume going forward that all
    of $a$, $b$, $c$ and $d$ are positive.

    Now we separate into two cases. The first case we consider is the case in
    which $a/b$ and $c/d$ belong to the same closed binade---that is, there's
    an integer~$e$ such that both $a/b$ and $c/d$ lie in the interval $[2^e,
    2^{e+1}]$.
    Since consecutive IEEE 754 binary64 floats in that interval have
    difference~$2^{e-52}$, for $a/b$ and $c/d$ to round to the same float we
    must have
    $\abs{a/b - c/d} \le 2^{e-52}$, from which
    \begin{equation}
        2^{52-e}\abs{ad - bc} \le bd.\label{ineq:1}
    \end{equation}
    From this inequality combined with $2^e \le a/b$ and $2^e \le c/d$, we
    have:
    \begin{equation}
        2^{52+e}\abs{ad - bc} \le 2^{2e}bd \le ac  .\label{ineq:2}
    \end{equation}
    Using (\ref{ineq:1}) if $e \le 0$ and (\ref{ineq:2}) if $e \ge 0$, along
    with the bound on~$\max(a, b, c, d)$, we have
    \begin{equation}
        2^{52 + \abs{e}}\abs{ad - bc} \le 67114657^2 < 2^{53}.\label{ineq:3}
    \end{equation}
    hence
    \begin{equation}
        2^{\abs{e}}\abs{ad - bc} < 2.\label{ineq:4}
    \end{equation}
    It follows that either $\abs{ad - bc} = 0$ (in which case $a/b = c/d$ as
    required), or $\abs{ad - bc} = 1$ and $e = 0$. In this case the inequality
    (\ref{ineq:1}) gives $2^{52} \le bd$, and the inequalities $2^e \le a/b$
    and $2^e \le c/d$ give $b \le a$ and $c \le d$. At this point we look for
    a contradiction.

    Swapping $a/b$ and $c/d$ if necessary, we can assume that $d \le b$, so
    from $2^{52} \le bd$ we have $2^{26} \le b \le a$. Now it's possible to do
    an exhaustive search over all pairs $(a, b)$ of integers satisfying
    $$ 2^{26} \le b \le a \le 67114657.$$ There are exactly $16788115$ such
    pairs (reducing to $10204542$ after we discard those with $\gcd(a, b) \ne
    1$), making this search computationally very feasible. For each pair $(a,
    b)$ we can use the extended Euclidean algorithm to efficiently find all
    possible solutions in integers $c$ and $d$ to $\abs{ad - bc} = 1$ with $0 <
    d \le b$ (there are at most two), and check that $a/b$ and $c/d$ do not
    round to the same float, giving us our contradiction.

    There remains the second case, where there is no integer $e$ such that
    both $a/b$ and $c/d$ lie in $[2^e, 2^{e+1}]$. The only way for this to
    be possible is if there's a power of two separating $a/b$ and $c/d$; that
    is, without loss of generality (swapping $a/b$ and $c/d$ if necessary)
    there's an $e$ satisfying
    $$a/b < 2^e < c/d.$$
    From the bounds on $a$, $b$, $c$ and~$d$, we must have
    $-26 \le e \le 26$. But now $2^e$ can be expressed as a fraction with
    numerator and denominator not exceeding $67114657$, and since $a/b$ and
    $c/d$ round to the same float, $2^e$ (being squeezed between $a/b$ and
    $c/d$) must round to that same float. So we can apply the case 1 proof to
    $a/b$ and $2^e$ to deduce that $a/b = 2^e$, and again to $2^e$ and $c/d$ to
    deduce that $2^e = c/d$, hence that $a/b = c/d$, as required.
\end{proof}

\end{document}
